<http://www.bbc.co.uk/ontologies/politics/governsGSS>
      a       <http://www.w3.org/2002/07/owl#ObjectProperty> ;
      <http://www.w3.org/2000/01/rdf-schema#comment>
              "property to relate a political organisation, such as a Council, to the area of Statistical Geography which it governs."@en-gb ;
      <http://www.w3.org/2000/01/rdf-schema#isDefinedBy>
              <http://www.bbc.co.uk/ontologies/politics> ;
      <http://www.w3.org/2000/01/rdf-schema#label>
              "governsGSS"@en-gb .

<http://www.bbc.co.uk/ontologies/politics/Council>
      a       <http://www.w3.org/2002/07/owl#Class> ;
      <http://www.w3.org/2000/01/rdf-schema#comment>
              "An organization with a formal role in local administration or government."@en-gb ;
      <http://www.w3.org/2000/01/rdf-schema#isDefinedBy>
              <http://www.bbc.co.uk/ontologies/politics> ;
      <http://www.w3.org/2000/01/rdf-schema#label>
              "Council"@en-gb ;
      <http://www.w3.org/2000/01/rdf-schema#subClassOf>
              <http://www.bbc.co.uk/ontologies/coreconcepts/Organisation> .

<http://www.bbc.co.uk/ontologies/politics>
      a       <http://www.w3.org/2002/07/owl#Ontology> , <http://www.bbc.co.uk/ontologies/provenance/Ontology> ;
      <http://www.w3.org/2000/01/rdf-schema#comment>
              "An ontology which describes a model for politics, specifically in terms of local government and elections. This is an evolving spec, originally designed to cope with UK (England and Northern Ireland) Local, and European Elections in May 2014."@en-gb ;
      <http://www.w3.org/2000/01/rdf-schema#label>
              "Politics Ontology"@en-gb ;
      <http://purl.org/dc/elements/1.1/creator>
              <http://www.r4isstatic.com/> ;
      <http://purl.org/dc/elements/1.1/date>
              "2014-01-06"^^<http://www.w3.org/2001/XMLSchema#date> ;
      <http://purl.org/dc/terms/license>
              <http://creativecommons.org/licenses/by/4.0/> ;
      <http://www.bbc.co.uk/ontologies/provenance/canonicalLocation>
              "https://repo.dev.bbc.co.uk/services/linked-data/ontologies/domain/news/politics-ontology-0.7.ttl"^^<http://www.w3.org/2001/XMLSchema#string> ;
      <http://www.bbc.co.uk/ontologies/provenance/changeReason>
              "Adding Constituency class."@en-gb ;
      <http://www.bbc.co.uk/ontologies/provenance/provided>
              "2014-12-11T10:19:52+00:00"^^<http://www.w3.org/2001/XMLSchema#dateTime> ;
      <http://www.bbc.co.uk/ontologies/provenance/provider>
              <mailto:sam.starling@bbc.co.uk> ;
      <http://www.bbc.co.uk/ontologies/provenance/public>
              "true"^^<http://www.w3.org/2001/XMLSchema#boolean> ;
      <http://www.bbc.co.uk/ontologies/provenance/slug>
              "politics"^^<http://www.w3.org/2001/XMLSchema#string> ;
      <http://www.bbc.co.uk/ontologies/provenance/version>
              "0.7"^^<http://www.w3.org/2001/XMLSchema#string> ;
      <http://www.w3.org/2002/07/owl#imports>
              <http://www.bbc.co.uk/ontologies/coreconcepts> , <http://www.bbc.co.uk/ontologies/provenance> ;
      <http://www.w3.org/2002/07/owl#priorVersion>
              <http://www.bbc.co.uk/ontologies/politics/0.6> ;
      <http://www.w3.org/2002/07/owl#versionIRI>
              <http://www.bbc.co.uk/ontologies/politics/0.7> ;
      <http://www.w3.org/2002/07/owl#versionInfo>
              "0.7"@en-gb .

<http://www.bbc.co.uk/ontologies/politics/StatisticalGeography>
      a       <http://www.w3.org/2002/07/owl#Class> ;
      <http://www.w3.org/2000/01/rdf-schema#comment>
              "A type of geographical bounded area defined specifically to cover political boundaries."@en-gb ;
      <http://www.w3.org/2000/01/rdf-schema#isDefinedBy>
              <http://www.bbc.co.uk/ontologies/politics> ;
      <http://www.w3.org/2000/01/rdf-schema#label>
              "StatisticalGeography"@en-gb ;
      <http://www.w3.org/2000/01/rdf-schema#subClassOf>
              <http://www.bbc.co.uk/ontologies/coreconcepts/Place> .

<http://www.bbc.co.uk/ontologies/politics/PoliticalParty>
      a       <http://www.w3.org/2002/07/owl#Class> ;
      <http://www.w3.org/2000/01/rdf-schema#comment>
              "An organization which seeks to influence, direct, or entirely perform government policy, commonly with a shared vision, ideals and goals which unites its' members and supporters."@en-gb ;
      <http://www.w3.org/2000/01/rdf-schema#isDefinedBy>
              <http://www.bbc.co.uk/ontologies/politics> ;
      <http://www.w3.org/2000/01/rdf-schema#label>
              "Political Party"@en-gb ;
      <http://www.w3.org/2000/01/rdf-schema#subClassOf>
              <http://www.bbc.co.uk/ontologies/coreconcepts/Organisation> .

<http://www.bbc.co.uk/ontologies/politics/Election>
      a       <http://www.w3.org/2002/07/owl#Class> ;
      <http://www.w3.org/2000/01/rdf-schema#comment>
              "An event which encapsulates the formal decision-making process by which a population chooses an individual to hold public office."@en-gb ;
      <http://www.w3.org/2000/01/rdf-schema#isDefinedBy>
              <http://www.bbc.co.uk/ontologies/politics> ;
      <http://www.w3.org/2000/01/rdf-schema#label>
              "Election"@en-gb ;
      <http://www.w3.org/2000/01/rdf-schema#subClassOf>
              <http://www.bbc.co.uk/ontologies/coreconcepts/Event> .

<http://www.bbc.co.uk/ontologies/politics/Constituency>
      a       <http://www.w3.org/2002/07/owl#Class> ;
      <http://www.w3.org/2000/01/rdf-schema#comment>
              "An electoral area or division, which can be represented in a political institution."@en-gb ;
      <http://www.w3.org/2000/01/rdf-schema#isDefinedBy>
              <http://www.bbc.co.uk/ontologies/politics> ;
      <http://www.w3.org/2000/01/rdf-schema#label>
              "Constituency"@en-gb ;
      <http://www.w3.org/2000/01/rdf-schema#subClassOf>
              <http://www.bbc.co.uk/ontologies/politics/StatisticalGeography> .
