@prefix crs: <http://def.seegrid.csiro.au/isotc211/iso19111/2008/crs/> .
@prefix dc: <http://purl.org/dc/elements/1.1/> .
@prefix dcterms: <http://purl.org/dc/terms/> .
@prefix def: <http://www.opengis.net/def/> .
@prefix eo: <http://www.opengis.net/def/eo/> .
@prefix owl: <http://www.w3.org/2002/07/owl#> .
@prefix policy: <http://www.opengis.net/def/metamodel/ogc-na/> .
@prefix rdf: <http://www.w3.org/1999/02/22-rdf-syntax-ns#> .
@prefix rdfs: <http://www.w3.org/2000/01/rdf-schema#> .
@prefix skos: <http://www.w3.org/2004/02/skos/core#> .
@prefix xsd: <http://www.w3.org/2001/XMLSchema#> .
@prefix status: <http://www.opengis.net/def/status/> .
@prefix dcterms: <http://purl.org/dc/terms/> .

<http://www.opengis.net/def/uom>
  rdf:type skos:ConceptScheme ;
  rdfs:label "units of measure definitions"^^xsd:string ;
  skos:prefLabel "units of measure definitions" ;
    policy:collectionView <http://www.opengis.net/def/uom/> ;
.

<http://www.opengis.net/def/uom/>
  skos:member <http://www.opengis.net/def/uom/OGC/> ;
  skos:member <http://www.opengis.net/def/uom/UCUM/> ;
  rdf:type skos:Collection ;
  dc:source "ISO 10000"^^xsd:string ;
  dcterms:created "2012-02-14"^^xsd:date ;
  rdfs:label "units of measure" ;
  skos:member <http://www.opengis.net/def/uom/EPSG/> ;
  skos:member <http://www.opengis.net/def/uom/SI/> ;
.
<http://www.opengis.net/def/uom/EPSG/>
  rdf:type skos:Collection ;
  rdfs:label "EPSG units of measure"^^xsd:string ;
  owl:sameAs <http://www.opengis.net/def/uom/epsg/> ;

.
<http://www.opengis.net/def/uom/epsg/>
  rdf:type skos:Collection ;
.



<http://www.opengis.net/def/uom/OGC/>
  rdf:type skos:Collection ;
  dcterms:created "2012-02-14"^^xsd:date ;
  rdfs:label "OGC Units of Measure" ;
  owl:sameAs <http://www.opengis.net/def/uom/ogc/> ;
  skos:member <http://www.opengis.net/def/uom/OGC/1.0/> ;
.
<http://www.opengis.net/def/uom/OGC/1.0>
  owl:sameAs <http://www.opengis.net/def/uom/OGC/1.0/> ;
.
<http://www.opengis.net/def/uom/OGC/1.0/>
  rdf:type skos:Collection ;
  dcterms:created "2012-02-14"^^xsd:date ;
  rdfs:label "OGC Units of Measure 1.0" ;
  owl:sameAs <http://www.opengis.net/def/uom/ogc/1.0/> ;
  skos:member <http://www.opengis.net/def/uom/OGC/1.0/GridSpacing> ;
  skos:member <http://www.opengis.net/def/uom/OGC/1.0/degree> ;
  skos:member <http://www.opengis.net/def/uom/OGC/1.0/metre> ;
  skos:member <http://www.opengis.net/def/uom/OGC/1.0/radian> ;
  skos:member <http://www.opengis.net/def/uom/OGC/1.0/unity> ;
.
<http://www.opengis.net/def/uom/OGC/1.0/GridSpacing>
  rdf:type skos:Concept ;
  dc:creator "Arliss Whiteside" ;
  dc:date "2010-03-23" ;
  dcterms:created "2010-03-23" ;
  dcterms:modified "2012-02-14"^^xsd:date ;
  policy:status status:valid ;
  rdfs:label "grid spacing"@en ;
  owl:sameAs <http://www.opengis.net/def/uom/ogc/1.0/gridspacing> ;
  skos:definition "Spacing between adjacent grid lines, or between centers of adjacent pixels"@en ;
  skos:inScheme def:scheme ;
  skos:prefLabel "grid spacing"@en ;
.
<http://www.opengis.net/def/uom/OGC/1.0/degree>
  rdf:type skos:Concept ;
  dc:creator "Arliss Whiteside" ;
  dc:date "2010-03-23" ;
  dc:source "OGC 07-092r3 Table 9"^^xsd:string ;
  dcterms:created "2010-03-23" ;
  dcterms:modified "2012-02-14"^^xsd:date ;
  policy:status status:valid ;
  rdfs:label "degree"@en ;
  rdfs:seeAlso <http://www.opengis.net/doc/urn-def/1.3#Table-9> ;
  owl:sameAs <http://www.opengis.net/def/uom/UCUM/0/deg> ;
  owl:sameAs <http://www.opengis.net/def/uom/ogc/1.0/degree> ;
  skos:definition "Angular degree"@en ;
  skos:inScheme def:scheme ;
  skos:prefLabel "degree"@en ;
.
<http://www.opengis.net/def/uom/OGC/1.0/metre>
  rdf:type skos:Concept ;
  dc:creator "Arliss Whiteside" ;
  dc:date "2010-03-23" ;
  dc:source "OGC 07-092r3 Table 9"^^xsd:string ;
  dcterms:created "2010-03-23" ;
  dcterms:modified "2012-02-14"^^xsd:date ;
  policy:status status:valid ;
  rdfs:label "meter"@en-us ;
  rdfs:label "metre"@en ;
  rdfs:seeAlso <http://www.opengis.net/doc/urn-def/1.3#Table-9> ;
  owl:sameAs <http://www.opengis.net/def/uom/UCUM/0/m> ;
  owl:sameAs <http://www.opengis.net/def/uom/ogc/1.0/metre> ;
  skos:definition "The metre is the length of the path travelled by light in vacuum during a time interval of 1/299 792 458 of a second."@en ;
  skos:inScheme def:scheme ;
  skos:prefLabel "meter"@en-us ;
  skos:prefLabel "metre"@en ;
.
<http://www.opengis.net/def/uom/OGC/1.0/radian>
  rdf:type skos:Concept ;
  dc:creator "Arliss Whiteside" ;
  dc:date "2010-03-23" ;
  dc:source "OGC 07-092r3 Table 9"^^xsd:string ;
  dcterms:created "2010-03-23" ;
  dcterms:modified "2012-02-14"^^xsd:date ;
  policy:status status:valid ;
  rdfs:label "radian"@en ;
  rdfs:seeAlso <http://www.opengis.net/doc/urn-def/1.3#Table-9> ;
  owl:sameAs <http://www.opengis.net/def/uom/UCUM/0/radian> ;
  owl:sameAs <http://www.opengis.net/def/uom/ogc/1.0/radian> ;
  skos:definition "Angular radian"@en ;
  skos:inScheme def:scheme ;
  skos:prefLabel "radian"@en ;
.
<http://www.opengis.net/def/uom/OGC/1.0/unity>
  rdf:type skos:Concept ;
  dc:creator "Arliss Whiteside" ;
  dc:date "2010-03-23" ;
  dc:source "OGC 07-092r3 Table 9"^^xsd:string ;
  dcterms:created "2010-03-23" ;
  dcterms:modified "2012-02-14"^^xsd:date ;
  policy:status status:valid ;
  rdfs:label "unity"@en ;
  rdfs:seeAlso <http://www.opengis.net/doc/urn-def/1.3#Table-9> ;
  owl:sameAs <http://www.opengis.net/def/uom/ogc/1.0/unity> ;
  skos:definition "unitless ratio of two quantities with the same units"@en ;
  skos:inScheme def:scheme ;
  skos:prefLabel "unity"@en ;
.
<http://www.opengis.net/def/uom/UCUM>
  owl:sameAs <http://www.opengis.net/def/uom/UCUM/> ;
.
<http://www.opengis.net/def/uom/UCUM/>
  rdf:type skos:Collection ;
  dcterms:created "2012-02-14"^^xsd:date ;
  rdfs:label "UCUM Units of Measure" ;
  owl:sameAs <http://www.opengis.net/def/uom/ucum/> ;
  skos:member <http://www.opengis.net/def/uom/UCUM/0/> ;
.
<http://www.opengis.net/def/uom/UCUM/0>
  owl:sameAs <http://www.opengis.net/def/uom/UCUM/0/> ;
.
<http://www.opengis.net/def/uom/UCUM/0/>
  rdf:type skos:Collection ;
  dcterms:created "2012-02-14"^^xsd:date ;
  rdfs:label "UCUM Units of Measure 0" ;
  rdfs:seeAlso <http://aurora.regenstrief.org/~ucum/ucum.html> ;
  owl:sameAs <http://www.opengis.net/def/uom/ucum/0/> ;
.
<http://www.opengis.net/def/uom/ogc/>
  rdf:type skos:Collection ;
.
<http://www.opengis.net/def/uom/ogc/1.0/>
  rdf:type skos:Collection ;
.
<http://www.opengis.net/def/uom/ogc/1.0/degree>
  rdf:type skos:Concept ;
  policy:status status:valid ;
  owl:sameAs <http://www.opengis.net/def/uom/OGC/1.0/degree> ;
.
<http://www.opengis.net/def/uom/ogc/1.0/gridspacing>
  rdf:type skos:Concept ;
  policy:status status:valid ;
  owl:sameAs <http://www.opengis.net/def/uom/OGC/1.0/GridSpacing> ;
.
<http://www.opengis.net/def/uom/ogc/1.0/metre>
  rdf:type skos:Concept ;
  policy:status status:valid ;
  owl:sameAs <http://www.opengis.net/def/uom/OGC/1.0/metre> ;
.
<http://www.opengis.net/def/uom/ogc/1.0/radian>
  rdf:type skos:Concept ;
  policy:status status:valid ;
  owl:sameAs <http://www.opengis.net/def/uom/OGC/1.0/radian> ;
.
<http://www.opengis.net/def/uom/ogc/1.0/unity>
  rdf:type skos:Concept ;
  policy:status status:valid ;
  owl:sameAs <http://www.opengis.net/def/uom/OGC/1.0/unity> ;
.
<http://www.opengis.net/def/uom/ucum/>
  rdf:type skos:Collection ;
.
<http://www.opengis.net/def/uom/ucum/0/>
  rdf:type skos:Collection ;
.

<http://www.opengis.net/def/uom/si/>
  owl:sameAs <http://www.opengis.net/def/uom/SI/> ;
.

<http://www.opengis.net/def/uom/SI/>
  rdf:type skos:Collection ;
  rdfs:label "SI units of measure"^^xsd:string ;
  rdfs:seeAlso <http://www.bipm.org/en/si/> ;
  owl:sameAs <http://www.opengis.net/def/uom/si/> ;
  skos:member <http://www.opengis.net/def/uom/SI/ampere> ;
  skos:member <http://www.opengis.net/def/uom/SI/candela> ;
  skos:member <http://www.opengis.net/def/uom/SI/kelvin> ;
  skos:member <http://www.opengis.net/def/uom/SI/kilogram> ;
  skos:member <http://www.opengis.net/def/uom/SI/metre> ;
  skos:member <http://www.opengis.net/def/uom/SI/mole> ;
  skos:member <http://www.opengis.net/def/uom/SI/second> ;
.
<http://www.opengis.net/def/uom/SI/ampere>
  rdf:type skos:Concept ;
  rdfs:seeAlso <http://www.bipm.org/en/si/si_brochure/chapter2/2-1/ampere.html> ;
  skos:definition "The ampere is that constant current which, if maintained in two straight parallel conductors of infinite length, of negligible circular cross-section, and placed 1 m apart in vacuum, would produce between these conductors a force equal to 2 x 10â€“7 newton per metre of length."^^xsd:string ;
  skos:exactMatch <http://qudt.org/vocab/unit#Ampere> ;
  skos:notation "A"^^xsd:string ;
.
<http://www.opengis.net/def/uom/SI/candela>
  rdf:type skos:Concept ;
  rdfs:seeAlso <http://www.bipm.org/en/si/si_brochure/chapter2/2-1/candela.html> ;
  skos:definition "The candela is the luminous intensity, in a given direction, of a source that emits monochromatic radiation of frequency 540 x 1012 hertz and that has a radiant intensity in that direction of 1/683 watt per steradian."^^xsd:string ;
  skos:exactMatch <http://qudt.org/vocab/unit#Candela> ;
  skos:notation "cd"^^xsd:string ;
.
<http://www.opengis.net/def/uom/SI/kelvin>
  rdf:type skos:Concept ;
  rdfs:seeAlso <http://www.bipm.org/en/si/si_brochure/chapter2/2-1/kelvin.html> ;
  skos:definition "The kelvin, unit of thermodynamic temperature, is the fraction 1/273.16 of the thermodynamic temperature of the triple point of water."^^xsd:string ;
  skos:exactMatch <http://qudt.org/vocab/unit#Kelvin> ;
  skos:notation "K"^^xsd:string ;
.
<http://www.opengis.net/def/uom/SI/kilogram>
  rdf:type skos:Concept ;
  rdfs:seeAlso <http://www.bipm.org/en/si/si_brochure/chapter2/2-1/kilogram.html> ;
  skos:definition "The kilogram is the unit of mass; it is equal to the mass of the international prototype of the kilogram."^^xsd:string ;
  skos:exactMatch <http://qudt.org/vocab/unit#Kilogram> ;
  skos:notation "kg"^^xsd:string ;
.
<http://www.opengis.net/def/uom/SI/metre>
  rdf:type skos:Concept ;
  rdfs:seeAlso <http://www.bipm.org/en/si/si_brochure/chapter2/2-1/metre.html> ;
  skos:definition "The metre is the length of the path travelled by light in vacuum during a time interval of 1/299 792 458 of a second."^^xsd:string ;
  skos:exactMatch <http://qudt.org/vocab/unit#Meter> ;
  skos:notation "m"^^xsd:string ;
.
<http://www.opengis.net/def/uom/SI/mole>
  rdf:type skos:Concept ;
  rdfs:seeAlso <http://www.bipm.org/en/si/si_brochure/chapter2/2-1/mole.html> ;
  skos:definition """	1.	The mole is the amount of substance of a system which contains as many elementary entities as there are atoms in 0.012 kilogram of carbon 12.
2.	When the mole is used, the elementary entities must be specified and may be atoms, molecules, ions, electrons, other particles, or specified groups of such particles."""^^xsd:string ;
  skos:exactMatch <http://qudt.org/vocab/unit#Mole> ;
  skos:notation "mol"^^xsd:string ;
.
<http://www.opengis.net/def/uom/SI/second>
  rdf:type skos:Concept ;
  rdfs:seeAlso <http://www.bipm.org/en/si/si_brochure/chapter2/2-1/second.html> ;
  skos:definition "The second is the duration of 9 192 631 770 periods of the radiation corresponding to the transition between the two hyperfine levels of the ground state of the caesium 133 atom."^^xsd:string ;
  skos:exactMatch <http://qudt.org/vocab/unit#Second> ;
  skos:notation "s"^^xsd:string ;
.
